theories/aps_plus/examples/list_length.v
@@ -1,15 +1,15 @@
 From simuliris Require Import
   prelude.
-From simuliris.lambda_lang Require Export
+From simuliris.data_lang Require Export
   refinement.
-From simuliris.lambda_human_lang Require Export
+From simuliris.data_human_lang Require Export
   compilation.
-From simuliris.lambda_human_lang Require Import
+From simuliris.data_human_lang Require Import
   notations.
 From simuliris.aps_plus Require Import
   definition.
 
-Definition list_length : lambda_human_program := {[
+Definition list_length : data_human_program := {[
   "list_length" := (BNamed "arg", (
     match: ![𝟙] "arg" with
       NIL =>
@@ -17,10 +17,10 @@ Definition list_length : lambda_human_program := {[
     | CONS <>, "xs" =>
         1 + $"list_length" "xs"
     end
-  )%lambda_human_expr)
+  )%data_human_expr)
 ]}.
 
-Definition list_length_aps_plus : lambda_human_program := {[
+Definition list_length_aps_plus : data_human_program := {[
   "list_length" := (BNamed "arg", (
     match: ![𝟙] "arg" with
       NIL =>
@@ -30,7 +30,7 @@ Definition list_length_aps_plus : lambda_human_program := {[
         let: "arg" := "xs" in
         $"list_length_aps" ("acc", "arg")
     end
-  )%lambda_human_expr) ;
+  )%data_human_expr) ;
   "list_length_aps" := (BNamed "arg", (
     let: "acc" := ![𝟙] "arg" in
     let: "arg" := ![𝟚] "arg" in
@@ -42,16 +42,16 @@ Definition list_length_aps_plus : lambda_human_program := {[
         let: "arg" := "xs" in
         $"list_length_aps" ("acc'" + "acc", "arg")
     end
-  )%lambda_human_expr)
+  )%data_human_expr)
 ]}.
 
 Goal
   aps_plus
-    (lambda_human_program_compile list_length)
-    (lambda_human_program_compile list_length_aps_plus).
+    (data_human_program_compile list_length)
+    (data_human_program_compile list_length_aps_plus).
 Proof.
   rewrite /list_length /list_length_aps_plus.
-  rewrite /lambda_human_program_compile map_fmap_singleton fmap_insert map_fmap_singleton /=.
+  rewrite /data_human_program_compile map_fmap_singleton fmap_insert map_fmap_singleton /=.
   exists {["list_length" := "list_length_aps"]}; try set_solver.
   + intros * (<- & <-)%lookup_singleton_Some.
     rewrite lookup_insert.
@@ -64,16 +64,16 @@ Proof.
 Qed.
 
 (* Lemma list_length_aps_plus_sound : *)
-(*   lambda_program_refinement *)
-(*     (lambda_human_program_compile list_length) *)
-(*     (lambda_human_program_compile list_length_aps_plus). *)
+(*   data_program_refinement *)
+(*     (data_human_program_compile list_length) *)
+(*     (data_human_program_compile list_length_aps_plus). *)
 (* Proof. *)
 (*   rewrite /list_length /list_length_aps_plus. apply aps_plus_sound. *)
 (*   - split. *)
-(*     + apply lambda_human_program_compile_well_formed. *)
-(*       rewrite /lambda_human_program_well_formed map_Forall_singleton //. *)
-(*     + apply lambda_human_program_compile_scope. *)
-(*   - rewrite /lambda_human_program_compile map_fmap_singleton fmap_insert map_fmap_singleton /=. *)
+(*     + apply data_human_program_compile_well_formed. *)
+(*       rewrite /data_human_program_well_formed map_Forall_singleton //. *)
+(*     + apply data_human_program_compile_scope. *)
+(*   - rewrite /data_human_program_compile map_fmap_singleton fmap_insert map_fmap_singleton /=. *)
 (*     exists {["list_length" := "list_length_aps"]}; try set_solver. *)
 (*     + intros * (<- & <-)%lookup_singleton_Some. *)
 (*       rewrite lookup_insert. *)
