theories/data_lang/sim/definition.v
@@ -7,16 +7,16 @@ From simuliris.base_logic Require Export
   lib.sim.heap_bij.
 From simuliris.program_logic Require Export
   sim.definition.
-From simuliris.lambda_lang Require Export
+From simuliris.data_lang Require Export
   language.
 
 Import heap.notations.
 
 Definition sim_protocol Σ :=
-  sim_protocol (iPropI Σ) lambda_ectx_lang lambda_ectx_lang.
+  sim_protocol (iPropI Σ) data_ectx_lang data_ectx_lang.
 
 Class SimGpreS Σ := {
-  sim_GpreS_heap_GpreS : SimHeapGpreS Σ loc lambda_val loc lambda_val ;
+  sim_GpreS_heap_GpreS : SimHeapGpreS Σ loc data_val loc data_val ;
   sim_GpreS_heap_bij_GpreS : SimHeapBijGpreS Σ loc loc ;
 }.
 #[global] Arguments Build_SimGpreS _ {_ _} : assert.
@@ -24,13 +24,13 @@ Class SimGpreS Σ := {
 #[local] Existing Instance sim_GpreS_heap_bij_GpreS.
 
 Class SimGS Σ := {
-  sim_GS_heap_GS :> SimHeapGS Σ loc lambda_val loc lambda_val ;
+  sim_GS_heap_GS :> SimHeapGS Σ loc data_val loc data_val ;
   sim_GS_heap_bij_GS :> SimHeapBijGS Σ loc loc ;
 }.
 #[global] Arguments Build_SimGS _ {_ _} : assert.
 
 Definition sim_Σ := #[
-  sim_heap_Σ loc lambda_val loc lambda_val ;
+  sim_heap_Σ loc data_val loc data_val ;
   sim_heap_bij_Σ loc loc
 ].
 
@@ -42,34 +42,34 @@ Proof.
 Qed.
 
 Section sim_programs.
-  Context `{sim_programs : !SimPrograms lambda_ectx_lang lambda_ectx_lang}.
+  Context `{sim_programs : !SimPrograms data_ectx_lang data_ectx_lang}.
 
-  #[global] Instance lambda_val_bi_similar `{sim_heap_bij_GS : !SimHeapBijGS Σ loc loc} : BiSimilar (iProp Σ) lambda_val lambda_val :=
+  #[global] Instance data_val_bi_similar `{sim_heap_bij_GS : !SimHeapBijGS Σ loc loc} : BiSimilar (iProp Σ) data_val data_val :=
     Build_BiSimilar $ λ vₛ vₜ,
       match vₛ, vₜ with
-      | LambdaUnit, LambdaUnit =>
+      | DataUnit, DataUnit =>
           True
-      | LambdaIndex idx1, LambdaIndex idx2 =>
+      | DataIndex idx1, DataIndex idx2 =>
           ⌜idx1 = idx2⌝
-      | LambdaTag tagₛ, LambdaTag tagₜ =>
+      | DataTag tagₛ, DataTag tagₜ =>
           ⌜tagₛ = tagₜ⌝
-      | LambdaInt nₛ, LambdaInt nₜ =>
+      | DataInt nₛ, DataInt nₜ =>
           ⌜nₛ = nₜ⌝
-      | LambdaBool bₛ, LambdaBool bₜ =>
+      | DataBool bₛ, DataBool bₜ =>
           ⌜bₛ = bₜ⌝
-      | LambdaLoc lₛ, LambdaLoc lₜ =>
+      | DataLoc lₛ, DataLoc lₜ =>
           (lₛ +ₗ 0) ≈ (lₜ +ₗ 0) ∗
           (lₛ +ₗ 1) ≈ (lₜ +ₗ 1) ∗
           (lₛ +ₗ 2) ≈ (lₜ +ₗ 2)
-      | LambdaFunc funcₛ, LambdaFunc funcₜ =>
+      | DataFunc funcₛ, DataFunc funcₜ =>
           ⌜funcₛ = funcₜ ∧ funcₛ ∈ dom sim_progₛ⌝
       | _, _ =>
           False
       end%I.
 
-  #[global] Instance sim_state `{sim_GS : !SimGS Σ} : SimState (iProp Σ) lambda_ectx_lang lambda_ectx_lang :=
+  #[global] Instance sim_state `{sim_GS : !SimGS Σ} : SimState (iProp Σ) data_ectx_lang data_ectx_lang :=
     Build_SimState (
-      λ (σₛ σₜ : lambda_state),
+      λ (σₛ σₜ : data_state),
         sim_heap_interpₛ σₛ ∗
         sim_heap_interpₜ σₜ ∗
         sim_heap_bij_inv
