theories/tmc/examples/list_map.v
@@ -1,15 +1,15 @@
 From simuliris Require Import
   prelude.
-From simuliris.lambda_lang Require Export
+From simuliris.data_lang Require Export
   refinement.
-From simuliris.lambda_human_lang Require Export
+From simuliris.data_human_lang Require Export
   compilation.
-From simuliris.lambda_human_lang Require Import
+From simuliris.data_human_lang Require Import
   notations.
 From simuliris.tmc Require Import
   soundness.
 
-Definition list_map : lambda_human_program := {[
+Definition list_map : data_human_program := {[
   "list_map" := (BNamed "arg", (
     let: "fn" := ![𝟙] "arg" in
     let: "xs" := ![𝟚] "arg" in
@@ -17,13 +17,13 @@ Definition list_map : lambda_human_program := {[
       NIL =>
         NILₕ
     | CONS "x", "xs" =>
-        let: "y" := LambdaHumanCall "fn" "x" in
+        let: "y" := DataHumanCall "fn" "x" in
         CONSₕ "y" ($"list_map" ("fn", "xs"))
     end
-  )%lambda_human_expr)
+  )%data_human_expr)
 ]}.
 
-Definition list_map_tmc : lambda_human_program := {[
+Definition list_map_tmc : data_human_program := {[
   "list_map" := (BNamed "arg", (
     let: "fn" := ![𝟙] "arg" in
     let: "xs" := ![𝟚] "arg" in
@@ -31,14 +31,14 @@ Definition list_map_tmc : lambda_human_program := {[
       NIL =>
         NILₕ
     | CONS "x", "xs" =>
-        let: "y" := LambdaHumanCall "fn" "x" in
+        let: "y" := DataHumanCall "fn" "x" in
         let: "dst" := CONSₕ "y" #ₕ() in
         ( let: "arg" := ("fn", "xs") in
           $"list_map_dps" ("dst", 𝟚, "arg")
         ) ;;
         "dst"
     end
-  )%lambda_human_expr) ;
+  )%data_human_expr) ;
   "list_map_dps" := (BNamed "arg", (
     let: "dst_idx" := ![𝟙] "arg" in
     let: "idx" := ![𝟚] "dst_idx" in
@@ -50,26 +50,26 @@ Definition list_map_tmc : lambda_human_program := {[
       NIL =>
         "dst" <-["idx"]- NILₕ
     | CONS "x", "xs" =>
-        let: "y" := LambdaHumanCall "fn" "x" in
+        let: "y" := DataHumanCall "fn" "x" in
         let: "dst'" := CONSₕ "y" #ₕ() in
         "dst" <-["idx"]- "dst'" ;;
         let: "arg" := ("fn", "xs") in
         $"list_map_dps" ("dst'", 𝟚, "arg")
     end
-  )%lambda_human_expr)
+  )%data_human_expr)
 ]}.
 
 Lemma list_map_tmc_sound :
-  lambda_program_refinement
-    (lambda_human_program_compile list_map)
-    (lambda_human_program_compile list_map_tmc).
+  data_program_refinement
+    (data_human_program_compile list_map)
+    (data_human_program_compile list_map_tmc).
 Proof.
   rewrite /list_map /list_map_tmc. apply tmc_sound.
   - split.
-    + apply lambda_human_program_compile_well_formed.
-      rewrite /lambda_human_program_well_formed map_Forall_singleton //.
-    + apply lambda_human_program_compile_scope.
-  - rewrite /lambda_human_program_compile map_fmap_singleton fmap_insert map_fmap_singleton /=.
+    + apply data_human_program_compile_well_formed.
+      rewrite /data_human_program_well_formed map_Forall_singleton //.
+    + apply data_human_program_compile_scope.
+  - rewrite /data_human_program_compile map_fmap_singleton fmap_insert map_fmap_singleton /=.
     exists {["list_map" := "list_map_dps"]}; try set_solver.
     + intros * (<- & <-)%lookup_singleton_Some.
       rewrite lookup_insert.
