theories/data_human_lang/compilation.v
@@ -1,0 +1,139 @@
+From simuliris Require Import
+  prelude.
+From simuliris.data_lang Require Export
+  metatheory.
+From simuliris.data_lang Require Import
+  notations.
+From simuliris.data_human_lang Require Export
+  metatheory.
+
+Definition data_human_bindings := list binder.
+Implicit Types bdgs : data_human_bindings.
+
+Fixpoint data_human_bindings_lookup_aux i bdgs x :=
+  match bdgs with
+  | [] =>
+      None
+  | y :: bdgs =>
+      if bool_decide (y = BNamed x)
+      then Some i
+      else data_human_bindings_lookup_aux (S i) bdgs x
+  end.
+Definition data_human_bindings_lookup bdgs x :=
+  data_human_bindings_lookup_aux 0 bdgs x.
+
+Definition data_human_val_compile v :=
+  match v with
+  | DataHumanUnit =>
+      DataUnit
+  | DataHumanIndex idx =>
+      DataIndex idx
+  | DataHumanTag tag =>
+      DataTag tag
+  | DataHumanInt n =>
+      DataInt n
+  | DataHumanBool b =>
+      DataBool b
+  | DataHumanFunc func =>
+      DataFunc func
+  end.
+
+Fixpoint data_human_expr_compile bdgs e :=
+  match e with
+  | DataHumanVal v =>
+      DataVal (data_human_val_compile v)
+  | DataHumanVar x =>
+      from_option DataVar Fail%data_expr (data_human_bindings_lookup bdgs x)
+  | DataHumanLet x e1 e2 =>
+      DataLet
+        (data_human_expr_compile bdgs e1)
+        (data_human_expr_compile (x :: bdgs) e2)
+  | DataHumanCall e1 e2 =>
+      DataCall
+        (data_human_expr_compile bdgs e1)
+        (data_human_expr_compile bdgs e2)
+  | DataHumanUnop op e =>
+      DataUnop op
+        (data_human_expr_compile bdgs e)
+  | DataHumanBinop op e1 e2 =>
+      DataBinop op
+        (data_human_expr_compile bdgs e1)
+        (data_human_expr_compile bdgs e2)
+  | DataHumanIf e0 e1 e2 =>
+      DataIf
+        (data_human_expr_compile bdgs e0)
+        (data_human_expr_compile bdgs e1)
+        (data_human_expr_compile bdgs e2)
+  | DataHumanConstr tag e1 e2 =>
+      DataConstr tag
+        (data_human_expr_compile bdgs e1)
+        (data_human_expr_compile bdgs e2)
+  | DataHumanLoad e1 e2 =>
+      DataLoad
+        (data_human_expr_compile bdgs e1)
+        (data_human_expr_compile bdgs e2)
+  | DataHumanStore e1 e2 e3 =>
+      DataStore
+        (data_human_expr_compile bdgs e1)
+        (data_human_expr_compile bdgs e2)
+        (data_human_expr_compile bdgs e3)
+  end.
+
+Definition data_human_program_compile (prog : data_human_program) : data_program :=
+  (λ '(x, e), data_human_expr_compile [x] e) <$> prog.
+
+Lemma data_human_val_compile_well_formed prog v :
+  data_human_program_well_formed prog →
+  data_human_val_well_formed prog v →
+  data_val_well_formed (data_human_program_compile prog) (data_human_val_compile v).
+Proof.
+  intros Hprog Hv. destruct v; try done. rewrite /= dom_fmap_L //.
+Qed.
+Lemma data_human_expr_compile_well_formed prog bdgs e :
+  data_human_program_well_formed prog →
+  data_human_expr_well_formed prog e →
+  data_expr_well_formed (data_human_program_compile prog) (data_human_expr_compile bdgs e).
+Proof.
+  intros Hprog He. revert bdgs. induction e; intros bdgs; try naive_solver; simpl.
+  - apply data_human_val_compile_well_formed; done.
+  - destruct (data_human_bindings_lookup bdgs _); done.
+Qed.
+Lemma data_human_program_compile_well_formed prog :
+  data_human_program_well_formed prog →
+  data_program_well_formed (data_human_program_compile prog).
+Proof.
+  intros Hprog. apply map_Forall_lookup. intros func ? ((x & e) & <- & Hfunc)%lookup_fmap_Some.
+  apply data_human_expr_compile_well_formed; first done.
+  rewrite /data_human_program_well_formed map_Forall_lookup in Hprog. naive_solver.
+Qed.
+
+Lemma data_human_bindings_lookup_aux_Some i bdgs x j :
+  data_human_bindings_lookup_aux i bdgs x = Some j →
+  i ≤ j < i + length bdgs.
+Proof.
+  revert i. induction bdgs as [| bdg bdgs]; simpl; intros i Hlookup; first done.
+  case_bool_decide.
+  - naive_solver lia.
+  - apply IHbdgs in Hlookup. lia.
+Qed.
+Lemma data_human_bindings_lookup_Some bdgs x i :
+  data_human_bindings_lookup bdgs x = Some i →
+  i < length bdgs.
+Proof.
+  apply data_human_bindings_lookup_aux_Some.
+Qed.
+
+Lemma data_human_expr_compile_scope scope bdgs e :
+  length bdgs = scope →
+  data_expr_scope scope (data_human_expr_compile bdgs e).
+Proof.
+  revert scope bdgs. induction e; simpl; intros scope bdgs Hlength; try naive_solver.
+  destruct (data_human_bindings_lookup _ _) eqn:Hlookup; last done.
+  rewrite -Hlength. eapply data_human_bindings_lookup_Some. done.
+Qed.
+Lemma data_human_program_compile_scope prog :
+  data_program_scope (data_human_program_compile prog).
+Proof.
+  apply map_Forall_lookup. intros func ? ((x & e) & <- & Hfunc)%lookup_fmap_Some.
+  apply data_human_expr_compile_scope. done.
+Qed.
