theories/data_human_lang/metatheory.v
@@ -1,0 +1,50 @@
+From simuliris Require Import
+  prelude.
+From simuliris.data_human_lang Require Export
+  syntax.
+
+Implicit Types prog : data_human_program.
+
+Definition data_human_val_well_formed prog v :=
+  match v with
+  | DataHumanFunc func =>
+      func ∈ dom prog
+  | _ =>
+      True
+  end.
+
+Fixpoint data_human_expr_well_formed prog e :=
+  match e with
+  | DataHumanVal v =>
+      data_human_val_well_formed prog v
+  | DataHumanVar _ =>
+      True
+  | DataHumanLet _ e1 e2 =>
+      data_human_expr_well_formed prog e1 ∧
+      data_human_expr_well_formed prog e2
+  | DataHumanCall e1 e2 =>
+      data_human_expr_well_formed prog e1 ∧
+      data_human_expr_well_formed prog e2
+  | DataHumanUnop _ e =>
+      data_human_expr_well_formed prog e
+  | DataHumanBinop _ e1 e2 =>
+      data_human_expr_well_formed prog e1 ∧
+      data_human_expr_well_formed prog e2
+  | DataHumanIf e0 e1 e2 =>
+      data_human_expr_well_formed prog e0 ∧
+      data_human_expr_well_formed prog e1 ∧
+      data_human_expr_well_formed prog e2
+  | DataHumanConstr _ e1 e2 =>
+      data_human_expr_well_formed prog e1 ∧
+      data_human_expr_well_formed prog e2
+  | DataHumanLoad e1 e2 =>
+      data_human_expr_well_formed prog e1 ∧
+      data_human_expr_well_formed prog e2
+  | DataHumanStore e1 e2 e3 =>
+      data_human_expr_well_formed prog e1 ∧
+      data_human_expr_well_formed prog e2 ∧
+      data_human_expr_well_formed prog e3
+  end.
+
+Definition data_human_program_well_formed prog :=
+  map_Forall (λ _ '(_, e), data_human_expr_well_formed prog e) prog.
