theories/data_human_lang/notations.v
@@ -1,0 +1,126 @@
+From simuliris Require Import
+  prelude.
+From simuliris.data_lang Require Export
+  notations.
+From simuliris.data_human_lang Require Export
+  syntax.
+
+Coercion DataHumanIndex : data_index >-> data_human_val.
+Coercion DataHumanTag : data_tag >-> data_human_val.
+Coercion DataHumanInt : Z >-> data_human_val.
+Coercion DataHumanBool : bool >-> data_human_val.
+
+Coercion DataHumanVal : data_human_val >-> data_human_expr.
+Coercion DataHumanVar : data_human_name >-> data_human_expr.
+Coercion DataHumanCall : data_human_expr >-> Funclass.
+
+Declare Scope data_human_val_scope.
+Delimit Scope data_human_val_scope with data_human_val.
+Bind Scope data_human_val_scope with data_human_val.
+
+Notation "()" := DataHumanUnit
+: data_human_val_scope.
+
+Declare Scope data_human_expr_scope.
+Delimit Scope data_human_expr_scope with data_human_expr.
+Bind Scope data_human_expr_scope with data_human_expr.
+
+Notation "#ₕ v" := (DataHumanVal v%Z%data_human_val%stdpp)
+( at level 5,
+  format "#ₕ v"
+).
+
+Notation "'Fail'" := (#ₕ() #ₕ())%data_human_expr
+: data_human_expr_scope.
+
+Notation "$ x" := (DataHumanFunc x)
+( at level 5,
+  format "$ x"
+) : data_human_expr_scope.
+
+Notation "'let:' x := e1 'in' e2" := (DataHumanLet x%binder e1%data_human_expr e2%data_human_expr)
+( at level 200,
+  x at level 1,
+  e1, e2 at level 200,
+  format "'[v' 'let:'  x  :=  '[' e1 ']'  'in' '/' e2 ']'"
+) : data_human_expr_scope.
+Notation "e1 ;; e2" := (DataHumanLet BAnon e1%data_human_expr e2%data_human_expr)
+( at level 100,
+  e2 at level 200,
+  format "'[v' '[hv' '[' e1 ']'  ;; ']' '/' e2 ']'"
+) : data_human_expr_scope.
+
+Notation "~ e" := (DataHumanUnop DataOpNeg e%data_human_expr)
+: data_human_expr_scope.
+Notation "- e" := (DataHumanUnop DataOpUminus e%data_human_expr)
+: data_human_expr_scope.
+
+Notation "e1 + e2" := (DataHumanBinop DataOpPlus e1%data_human_expr e2%data_human_expr)
+: data_human_expr_scope.
+Notation "e1 - e2" := (DataHumanBinop DataOpMinus e1%data_human_expr e2%data_human_expr)
+: data_human_expr_scope.
+Notation "e1 * e2" := (DataHumanBinop DataOpMult e1%data_human_expr e2%data_human_expr)
+: data_human_expr_scope.
+Notation "e1 `quot` e2" := (DataHumanBinop DataOpQuot e1%data_human_expr e2%data_human_expr)
+: data_human_expr_scope.
+Notation "e1 `rem` e2" := (DataHumanBinop DataOpRem e1%data_human_expr e2%data_human_expr)
+: data_human_expr_scope.
+Notation "e1 ≤ e2" := (DataHumanBinop DataOpLe e1%data_human_expr e2%data_human_expr)
+: data_human_expr_scope.
+Notation "e1 < e2" := (DataHumanBinop DataOpLt e1%data_human_expr e2%data_human_expr)
+: data_human_expr_scope.
+Notation "e1 = e2" := (DataHumanBinop DataOpEq e1%data_human_expr e2%data_human_expr)
+: data_human_expr_scope.
+Notation "e1 ≠ e2" := (~ (e1 = e2))%data_human_expr
+: data_human_expr_scope.
+
+Notation "'if:' e0 'then' e1 'else' e2" := (DataHumanIf e0%data_human_expr e1%data_human_expr e2%data_human_expr)
+( at level 200,
+  e0, e1, e2 at level 200
+) : data_human_expr_scope.
+Notation "e1 && e2" := (if: e1 then e2 else #ₕfalse)%data_human_expr
+( only parsing
+) : data_human_expr_scope.
+Notation "e1 || e2" := (if: e1 then #ₕtrue else e2)%data_human_expr
+( only parsing
+) : data_human_expr_scope.
+
+Notation "& tag" := (DataHumanConstr tag)
+( at level 5,
+  format "& tag"
+) : data_human_expr_scope.
+
+Notation "![ e2 ] e1" := (DataHumanLoad e1%data_human_expr e2%data_human_expr)
+( at level 9,
+  right associativity,
+  format "![ e2 ]  e1"
+) : data_human_expr_scope.
+Notation "! e" := (DataHumanLoad e%data_human_expr 𝟘)
+( at level 9,
+  right associativity,
+  format "! e"
+) : data_human_expr_scope.
+
+Notation "e1 <-[ e2 ]- e3" := (DataHumanStore e1%data_human_expr e2%data_human_expr e3%data_human_expr)
+( at level 20,
+  format "e1  <-[ e2 ]-  e3"
+) : data_human_expr_scope.
+
+Notation "( e1 , e2 , .. , en )" := (&data_tag_pair .. (&data_tag_pair e1 e2) .. en)%data_human_expr
+: data_human_expr_scope.
+
+Notation NILₕ := (&data_tag_nil #ₕ() #ₕ())%data_human_expr (only parsing).
+Notation CONSₕ := (&data_tag_cons)%data_human_expr (only parsing).
+Notation "'match:' e0 'with' 'NIL' => e1 | 'CONS' x , y => e2 'end'" := (
+  let: "__match" := e0 in
+  if: !"__match" = data_tag_nil then (
+    e1
+  ) else (
+    let: y := ![𝟚] "__match" in
+    let: x := ![𝟙] "__match" in
+    e2
+  )
+)%data_human_expr (
+  only parsing,
+  e0, e1, x, y, e2 at level 200
+) : data_human_expr_scope.
