theories/data_human_lang/syntax.v
@@ -1,0 +1,130 @@
+From stdpp Require Export
+  binders.
+
+From simuliris Require Import
+  prelude.
+From simuliris.data_lang Require Export
+  syntax.
+
+Notation data_human_name := string (only parsing).
+
+Inductive data_human_val :=
+  | DataHumanUnit
+  | DataHumanIndex (idx : data_index)
+  | DataHumanTag (tag : data_tag)
+  | DataHumanInt (n : Z)
+  | DataHumanBool (b : bool)
+  | DataHumanFunc (func : data_function).
+
+#[global] Instance data_human_val_inhabited : Inhabited data_human_val :=
+  populate DataHumanUnit.
+#[global] Instance data_human_val_eq_dec : EqDecision data_human_val :=
+  ltac:(solve_decision).
+#[global] Instance data_human_val_countable :
+  Countable data_human_val.
+Proof.
+  pose encode v :=
+    match v with
+    | DataHumanUnit =>
+        inl ()
+    | DataHumanIndex idx =>
+        inr $ inl idx
+    | DataHumanTag tag =>
+        inr $ inr $ inl tag
+    | DataHumanInt n =>
+        inr $ inr $ inr $ inl n
+    | DataHumanBool b =>
+        inr $ inr $ inr $ inr $ inl b
+    | DataHumanFunc func =>
+        inr $ inr $ inr $ inr $ inr func
+    end.
+  pose decode v :=
+    match v with
+    | inl () =>
+        DataHumanUnit
+    | inr (inl idx) =>
+        DataHumanIndex idx
+    | inr (inr (inl tag)) =>
+        DataHumanTag tag
+    | inr (inr (inr (inl n))) =>
+        DataHumanInt n
+    | inr (inr (inr (inr (inl b)))) =>
+        DataHumanBool b
+    | inr (inr (inr (inr (inr func)))) =>
+        DataHumanFunc func
+    end.
+  apply (inj_countable' encode decode). intros []; done.
+Qed.
+
+Inductive data_human_expr :=
+  | DataHumanVal (v : data_human_val)
+  | DataHumanVar (x : data_human_name)
+  | DataHumanLet (x : binder) (e1 e2 : data_human_expr)
+  | DataHumanCall (e1 e2 : data_human_expr)
+  | DataHumanUnop (op : data_unop) (e : data_human_expr)
+  | DataHumanBinop (op : data_binop) (e1 e2 : data_human_expr)
+  | DataHumanIf (e0 e1 e2 : data_human_expr)
+  | DataHumanConstr (tag : data_tag) (e1 e2 : data_human_expr)
+  | DataHumanLoad (e1 e2 : data_human_expr)
+  | DataHumanStore (e1 e2 e3 : data_human_expr).
+
+#[global] Instance data_human_expr_inhabited : Inhabited data_human_expr :=
+  populate (DataHumanVal inhabitant).
+#[global] Instance data_human_expr_eq_dec : EqDecision data_human_expr :=
+  ltac:(solve_decision).
+#[global] Instance data_human_expr_countable :
+  Countable data_human_expr.
+Proof.
+  pose fix encode e :=
+    match e with
+    | DataHumanVal v =>
+        GenLeaf (inl v)
+    | DataHumanVar x =>
+        GenLeaf (inr $ inl $ BNamed x)
+    | DataHumanLet x e1 e2 =>
+        GenNode 0 [GenLeaf (inr $ inl x); encode e1; encode e2]
+    | DataHumanCall e1 e2 =>
+        GenNode 1 [encode e1; encode e2]
+    | DataHumanUnop op e =>
+        GenNode 2 [GenLeaf (inr $ inr $ inl op); encode e]
+    | DataHumanBinop op e1 e2 =>
+        GenNode 3 [GenLeaf (inr $ inr $ inr $ inl op); encode e1; encode e2]
+    | DataHumanIf e0 e1 e2 =>
+        GenNode 4 [encode e0; encode e1; encode e2]
+    | DataHumanConstr tag e1 e2 =>
+        GenNode 5 [GenLeaf (inr $ inr $ inr $ inr tag); encode e1; encode e2]
+    | DataHumanLoad e1 e2 =>
+        GenNode 6 [encode e1; encode e2]
+    | DataHumanStore e1 e2 e3 =>
+        GenNode 7 [encode e1; encode e2; encode e3]
+    end.
+  pose fix decode e :=
+    match e with
+    | GenLeaf (inl v) =>
+        DataHumanVal v
+    | GenLeaf (inr (inl (BNamed x))) =>
+        DataHumanVar x
+    | GenNode 0 [GenLeaf (inr (inl x)); e1; e2] =>
+        DataHumanLet x (decode e1) (decode e2)
+    | GenNode 1 [e1; e2] =>
+        DataHumanCall (decode e1) (decode e2)
+    | GenNode 2 [GenLeaf (inr (inr (inl op))); e] =>
+        DataHumanUnop op (decode e)
+    | GenNode 3 [GenLeaf (inr (inr (inr (inl op)))); e1; e2] =>
+        DataHumanBinop op (decode e1) (decode e2)
+    | GenNode 4 [e0; e1; e2] =>
+        DataHumanIf (decode e0) (decode e1) (decode e2)
+    | GenNode 5 [GenLeaf (inr (inr (inr (inr tag)))); e1; e2] =>
+        DataHumanConstr tag (decode e1) (decode e2)
+    | GenNode 6 [e1; e2] =>
+        DataHumanLoad (decode e1) (decode e2)
+    | GenNode 7 [e1; e2; e3] =>
+        DataHumanStore (decode e1) (decode e2) (decode e3)
+    | _ =>
+        @inhabitant _ data_human_expr_inhabited
+    end.
+  apply (inj_countable' encode decode). intros e. induction e; simpl; congruence.
+Qed.
+
+Definition data_human_program :=
+  gmap data_function (binder * data_human_expr).
