theories/data_lang/ectx_decompositions.v
@@ -1,0 +1,110 @@
+From simuliris Require Import
+  prelude.
+From simuliris.common Require Import
+  tactics.
+From simuliris.data_lang Require Export
+  language.
+
+Fixpoint data_ectx_decompositions e :=
+  let data_ectx_decompositions_with k e :=
+    (λ '(K, e), ([k] ⋅ K, e)) <$> data_ectx_decompositions e
+  in
+  ([], e) ::
+  match e with
+  | DataVar _
+  | DataVal _
+  | DataBinop _ _ _
+  | DataBinopDet _ _ _
+  | DataConstr _ _ _
+  | DataConstrDet _ _ _ =>
+      []
+  | DataLet e1 e2 =>
+      data_ectx_decompositions_with (DataEctxiLet e2) e1
+  | DataCall e1 e2 =>
+      data_ectx_decompositions_with (DataEctxiCall1 e1) e2 ++
+      match data_to_val e2 with
+      | None => []
+      | Some v2 =>
+          data_ectx_decompositions_with (DataEctxiCall2 v2) e1
+      end
+  | DataUnop op e =>
+      data_ectx_decompositions_with (DataEctxiUnop op) e
+  | DataIf e0 e1 e2 =>
+      data_ectx_decompositions_with (DataEctxiIf e1 e2) e0
+  | DataLoad e1 e2 =>
+      data_ectx_decompositions_with (DataEctxiLoad1 e1) e2 ++
+      match data_to_val e2 with
+      | None => []
+      | Some v2 =>
+          data_ectx_decompositions_with (DataEctxiLoad2 v2) e1
+      end
+  | DataStore e1 e2 e3 =>
+      data_ectx_decompositions_with (DataEctxiStore1 e1 e2) e3 ++
+      match data_to_val e3 with
+      | None => []
+      | Some v3 =>
+          data_ectx_decompositions_with (DataEctxiStore2 e1 v3) e2 ++
+          match data_to_val e2 with
+          | None => []
+          | Some v2 =>
+              data_ectx_decompositions_with (DataEctxiStore3 v2 v3) e1
+          end
+      end
+  end.
+
+Lemma data_ectx_decompositions_sound e K e' :
+  (K, e') ∈ data_ectx_decompositions e →
+  e = K @@ e'.
+Proof.
+  revert K e'. induction e; simpl; intros;
+    repeat match goal with
+    | _ =>
+        progress decompose_elem_of_list
+    | H : _ ∈ _ <$> _ |- _ =>
+        apply elem_of_list_fmap in H as ([] & ? & ?); simplify
+    | H : _ ∈ match data_to_val ?e with None => _ | Some _ => _ end |- _ =>
+        let Heq := fresh "Heq" in
+        destruct (data_to_val e) eqn:Heq; first apply of_to_val in Heq
+    end;
+    rewrite -?fill_op; naive_solver.
+Qed.
+
+Lemma data_ectx_decompositions_base e :
+  (∅, e) ∈ data_ectx_decompositions e.
+Proof.
+  destruct e; econstructor.
+Qed.
+
+Lemma data_ectx_decompositions_complete K e :
+  (K, e) ∈ data_ectx_decompositions (K @@ e).
+Proof.
+  revert K e.
+  assert (∀ K e, (reverse K, e) ∈ data_ectx_decompositions ((reverse K) @@ e)).
+  { intros. induction K as [| k K]; first apply data_ectx_decompositions_base.
+    rewrite reverse_cons -fill_op /=. destruct k; simpl;
+    repeat match goal with
+    | |- _ ∈ _ :: _ =>
+        econstructor
+    | |- _ ∈ _ <$> _ =>
+        apply elem_of_list_fmap; by exists (reverse K, e)
+    | |- _ ∈ _ ++ _ =>
+        apply elem_of_app; left
+    | _ =>
+        simpl
+    end.
+  }
+  intros. by rewrite -(reverse_involutive K).
+Qed.
+Lemma data_ectx_decompositions_complete' e K e' :
+  e = K @@ e' →
+  (K, e') ∈ data_ectx_decompositions e.
+Proof.
+  intros ->. apply data_ectx_decompositions_complete.
+Qed.
+
+Lemma data_ectx_decompositions_spec e K e' :
+  e = K @@ e' ↔
+  (K, e') ∈ data_ectx_decompositions e.
+Proof.
+  split; eauto using data_ectx_decompositions_sound, data_ectx_decompositions_complete'.
+Qed.
