theories/data_lang/language.v
@@ -1,0 +1,88 @@
+From simuliris Require Import
+  prelude.
+From simuliris.common Require Import
+  tactics.
+From simuliris.program_logic Require Export
+  ectxi_language.
+From simuliris.data_lang Require Export
+  semantics.
+
+Implicit Types l : loc.
+Implicit Types v w : data_val.
+Implicit Types e : data_expr.
+Implicit Types σ : data_state.
+
+Notation data_of_val := DataVal.
+
+Definition data_to_val e :=
+  match e with
+  | DataVal v => Some v
+  | _ => None
+  end.
+
+Canonical data_val_O := leibnizO data_val.
+Canonical data_expr_O := leibnizO data_expr.
+Canonical data_state_O := leibnizO data_state.
+
+Inductive data_ectxi :=
+  | DataEctxiLet e2
+  | DataEctxiCall1 e1
+  | DataEctxiCall2 v2
+  | DataEctxiUnop (op : data_unop)
+  | DataEctxiIf e1 e2
+  | DataEctxiLoad1 e1
+  | DataEctxiLoad2 v2
+  | DataEctxiStore1 e1 e2
+  | DataEctxiStore2 e1 v3
+  | DataEctxiStore3 v2 v3.
+
+Definition data_ectx := list data_ectxi.
+
+Definition data_fill_item k e :=
+  match k with
+  | DataEctxiLet e2 =>
+      DataLet e e2
+  | DataEctxiCall1 e1 =>
+      DataCall e1 e
+  | DataEctxiCall2 v2 =>
+      DataCall e (data_of_val v2)
+  | DataEctxiUnop op =>
+      DataUnop op e
+  | DataEctxiIf e1 e2 =>
+      DataIf e e1 e2
+  | DataEctxiLoad1 e1 =>
+      DataLoad e1 e
+  | DataEctxiLoad2 v2 =>
+      DataLoad e (data_of_val v2)
+  | DataEctxiStore1 e1 e2 =>
+      DataStore e1 e2 e
+  | DataEctxiStore2 e1 v3 =>
+      DataStore e1 e (data_of_val v3)
+  | DataEctxiStore3 v2 v3 =>
+      DataStore e (data_of_val v2) (data_of_val v3)
+  end.
+#[global] Instance data_ectxi_fill : Fill data_ectxi data_expr :=
+  Build_Fill data_fill_item.
+
+Lemma data_ectxi_lang_mixin :
+  EctxiLanguageMixin
+    data_of_val
+    data_to_val
+    data_head_step
+    data_ectxi.
+Proof.
+  split.
+  - naive_solver.
+  - intros []; naive_solver.
+  - intros * []; naive_solver.
+  - intros [] ?**; naive_solver.
+  - intros []; naive_solver.
+  - intros [] ? []; naive_solver.
+  - intros ? [] * Hstep; invert Hstep; naive_solver.
+Qed.
+Canonical data_ectxi_lang :=
+  Build_ectxi_language data_ectxi_lang_mixin.
+Canonical data_ectx_lang :=
+  ectx_language_of_ectxi_language data_ectxi_lang.
+Canonical data_lang :=
+  language_of_ectx_language data_ectx_lang.
