theories/data_lang/metatheory.v
@@ -1,0 +1,231 @@
+From simuliris Require Import
+  prelude.
+From simuliris.data_lang Require Export
+  syntax.
+
+Implicit Types prog : data_program.
+
+Definition data_val_well_formed prog v :=
+  match v with
+  | DataLoc _ =>
+      False
+  | DataFunc func =>
+      func ∈ dom prog
+  | _ =>
+      True
+  end.
+
+Fixpoint data_expr_well_formed prog e :=
+  match e with
+  | DataVal v =>
+      data_val_well_formed prog v
+  | DataVar _ =>
+      True
+  | DataLet e1 e2 =>
+      data_expr_well_formed prog e1 ∧
+      data_expr_well_formed prog e2
+  | DataCall e1 e2 =>
+      data_expr_well_formed prog e1 ∧
+      data_expr_well_formed prog e2
+  | DataUnop _ e =>
+      data_expr_well_formed prog e
+  | DataBinop _ e1 e2 =>
+      data_expr_well_formed prog e1 ∧
+      data_expr_well_formed prog e2
+  | DataBinopDet _ _ _ =>
+      False
+  | DataIf e0 e1 e2 =>
+      data_expr_well_formed prog e0 ∧
+      data_expr_well_formed prog e1 ∧
+      data_expr_well_formed prog e2
+  | DataConstr _ e1 e2 =>
+      data_expr_well_formed prog e1 ∧
+      data_expr_well_formed prog e2
+  | DataConstrDet _ _ _ =>
+      False
+  | DataLoad e1 e2 =>
+      data_expr_well_formed prog e1 ∧
+      data_expr_well_formed prog e2
+  | DataStore e1 e2 e3 =>
+      data_expr_well_formed prog e1 ∧
+      data_expr_well_formed prog e2 ∧
+      data_expr_well_formed prog e3
+  end.
+
+Fixpoint data_expr_scope scope e :=
+  match e with
+  | DataVal _ =>
+      True
+  | DataVar x =>
+      x < scope
+  | DataLet e1 e2 =>
+      data_expr_scope scope e1 ∧
+      data_expr_scope (S scope) e2
+  | DataCall e1 e2 =>
+      data_expr_scope scope e1 ∧
+      data_expr_scope scope e2
+  | DataUnop _ e =>
+      data_expr_scope scope e
+  | DataBinop _ e1 e2 =>
+      data_expr_scope scope e1 ∧
+      data_expr_scope scope e2
+  | DataBinopDet _ e1 e2 =>
+      data_expr_scope scope e1 ∧
+      data_expr_scope scope e2
+  | DataIf e0 e1 e2 =>
+      data_expr_scope scope e0 ∧
+      data_expr_scope scope e1 ∧
+      data_expr_scope scope e2
+  | DataConstr _ e1 e2 =>
+      data_expr_scope scope e1 ∧
+      data_expr_scope scope e2
+  | DataConstrDet _ e1 e2 =>
+      data_expr_scope scope e1 ∧
+      data_expr_scope scope e2
+  | DataLoad e1 e2 =>
+      data_expr_scope scope e1 ∧
+      data_expr_scope scope e2
+  | DataStore e1 e2 e3 =>
+      data_expr_scope scope e1 ∧
+      data_expr_scope scope e2 ∧
+      data_expr_scope scope e3
+  end.
+
+Definition data_program_well_formed prog :=
+  map_Forall (λ _, data_expr_well_formed prog) prog.
+
+Definition data_program_scope prog :=
+  map_Forall (λ _, data_expr_scope 1) prog.
+
+Definition data_program_valid prog :=
+  data_program_well_formed prog ∧ data_program_scope prog.
+
+Lemma subst_data_expr_scope ς1 ς2 scope e :
+  (∀ x, x < scope → ς1 x = ς2 x) →
+  data_expr_scope scope e →
+  e.[ς1] = e.[ς2].
+Proof.
+  revert ς1 ς2 scope. induction e as
+    [ v
+    | x
+    | e1 IHe1 e2 IHe2
+    | e1 IHe1 e2 IHe2
+    | e IHe
+    | e1 IHe1 e2 IHe2
+    | e1 IHe1 e2 IHe2
+    | e0 IHe0 e1 IHe1 e2 IHe2
+    | e1 IHe1 e2 IHe2
+    | e1 IHe1 e2 IHe2
+    | e1 IHe1 e2 IHe2
+    | e1 IHe1 e2 IHe2 e3 IHe3
+    ];
+    intros ς1 ς2 scope Hς Hscope;
+    asimpl;
+    try (f_equal; naive_solver).
+  f_equal; first naive_solver.
+  eapply IHe2; last naive_solver.
+  intros x Hx. destruct x; first done. asimpl. f_equal. naive_solver lia.
+Qed.
+Lemma subst_data_expr_scope_0 ς1 ς2 e :
+  data_expr_scope 0 e →
+  e.[ς1] = e.[ς2].
+Proof.
+  intros Hscope.
+  eapply subst_data_expr_scope; last done.
+  lia.
+Qed.
+Lemma subst_data_expr_scope_1 ς1 ς2 e :
+  ς1 0 = ς2 0 →
+  data_expr_scope 1 e →
+  e.[ς1] = e.[ς2].
+Proof.
+  intros Hς Hscope.
+  eapply subst_data_expr_scope; last done.
+  setoid_rewrite Nat.lt_1_r. naive_solver.
+Qed.
+Lemma subst_data_expr_scope_1' ς1 ς2 v e :
+  data_expr_scope 1 e →
+  e.[v .: ς1] = e.[v .: ς2].
+Proof.
+  apply subst_data_expr_scope_1. done.
+Qed.
+
+Lemma subst_data_program_scope ς1 ς2 prog func e :
+  ς1 0 = ς2 0 →
+  data_program_scope prog →
+  prog !! func = Some e →
+  e.[ς1] = e.[ς2].
+Proof.
+  intros Hσ Hwf Hlookup.
+  eapply subst_data_expr_scope_1; first done.
+  eapply map_Forall_lookup_1 in Hwf; naive_solver.
+Qed.
+Lemma subst_data_program_scope' ς1 ς2 v prog func e :
+  data_program_scope prog →
+  prog !! func = Some e →
+  e.[v .: ς1] = e.[v .: ς2].
+Proof.
+  apply subst_data_program_scope. done.
+Qed.
+
+Lemma data_expr_scope_le scope1 scope2 e :
+  scope1 ≤ scope2 →
+  data_expr_scope scope1 e →
+  data_expr_scope scope2 e.
+Proof.
+  revert scope1 scope2. elim e; try naive_solver lia.
+  intros e1 IH1 e2 IH2 scope1 scope2 Hscope (Hscope1 & Hscope2).
+  split; first naive_solver. eapply IH2; last done. lia.
+Qed.
+
+Lemma data_expr_scope_upn_subst_data_val n v scope e :
+  n < scope →
+  data_expr_scope scope e →
+  data_expr_scope (scope - 1) e.[upn n (DataVal v .: ids)].
+Proof.
+  revert n scope. induction e; intros n scope; try naive_solver; simpl.
+  - intros Hn Hx.
+    destruct (Nat.lt_ge_cases x n) as [Hx' | (dx & ->)%Nat.le_sum].
+    + rewrite upn_lt //=. lia.
+    + rewrite upn_ge; first lia.
+      rewrite Nat.sub_add'. destruct dx; first done. simpl. lia.
+  - intros Hn (Hscope1 & Hscope2). split; first naive_solver.
+    rewrite fold_up_upn.
+    destruct scope; first lia.
+    rewrite /= Nat.sub_0_r -(Nat.pred_succ (S scope)) -Nat.sub_1_r.
+    auto with lia.
+Qed.
+Lemma data_expr_scope_subst_data_val scope e v :
+  data_expr_scope scope e →
+  data_expr_scope (scope - 1) e.[DataVal v/].
+Proof.
+  destruct scope.
+  - intros Hscope%(data_expr_scope_le _ 1)%(data_expr_scope_upn_subst_data_val 0 v); naive_solver lia.
+  - apply (data_expr_scope_upn_subst_data_val 0). lia.
+Qed.
+
+Lemma data_expr_scope_ren ξ n scope e :
+  (∀ x, ξ x ≤ x + n) →
+  data_expr_scope scope e →
+  data_expr_scope (scope + n) e.[ren ξ].
+Proof.
+  revert scope ξ n. elim e; try naive_solver lia.
+  - intros x scope ξ n Hξ Hscope.
+    eapply (Nat.le_lt_trans _ (x + n)); naive_solver lia.
+  - intros e1 IH1 e2 IH2 scope ξ n Hξ (Hscope1 & Hscope2).
+    split; first naive_solver.
+    asimpl. rewrite -Nat.add_succ_l. apply IH2; last done.
+    intros []; simpl; [lia | rewrite -Nat.succ_le_mono //].
+Qed.
+Lemma data_expr_scope_lift n scope e :
+  data_expr_scope scope e →
+  data_expr_scope (scope + n) e.[ren (+n)].
+Proof.
+  apply data_expr_scope_ren. naive_solver lia.
+Qed.
+Lemma data_expr_scope_lift1 scope e :
+  data_expr_scope scope e →
+  data_expr_scope (S scope) e.[ren (+1)].
+Proof.
+  rewrite -Nat.add_1_r. apply data_expr_scope_lift.
+Qed.
