theories/data_lang/refinement.v
@@ -1,0 +1,17 @@
+From simuliris Require Import
+  prelude.
+From simuliris.program_logic Require Export
+  refinement.
+From simuliris.data_lang Require Export
+  language
+  metatheory.
+From simuliris.data_lang Require Import
+  notations.
+
+Definition data_program_refinement (progₛ progₜ : data_program) :=
+  map_Forall (λ (func : data_function) _,
+    ∀ vₛ vₜ : data_val,
+    data_val_well_formed progₛ vₛ →
+    vₛ ≈ vₜ →
+    expr_refinement progₛ progₜ (func vₛ) (func vₜ)
+  ) progₛ.
