theories/data_lang/rsim/definition.v
@@ -1,12 +1,12 @@
 From simuliris Require Import
   prelude.
-From simuliris.lambda_lang Require Export
+From simuliris.data_lang Require Export
   rsim.bisubst.
-From simuliris.lambda_lang Require Import
+From simuliris.data_lang Require Import
   sim.notations.
 
 Section sim_GS.
-  Context `{sim_programs : !SimPrograms lambda_ectx_lang lambda_ectx_lang}.
+  Context `{sim_programs : !SimPrograms data_ectx_lang data_ectx_lang}.
   Context `{sim_GS : !SimGS Σ}.
   Context (Χ : sim_protocol Σ).
   Implicit Types Γ : bisubst.
@@ -16,9 +16,9 @@ Section sim_GS.
     ⌜eₛ' = eₛ.[Γ.ₛ#] ∧ eₜ' = eₜ.[Γ.ₜ#]⌝ -∗
     bisubst_well_formed Γ -∗
     SIM eₛ' ≳ eₜ' [[ Χ ]] {{ Φ }}.
-  #[global] Arguments rsim _%I (_ _)%lambda_expr : assert.
+  #[global] Arguments rsim _%I (_ _)%data_expr : assert.
 
   Definition rsimv Φ eₛ eₜ : iProp Σ :=
     rsim (sim_post_vals Φ) eₛ eₜ.
-  #[global] Arguments rsimv _%I (_ _)%lambda_expr : assert.
+  #[global] Arguments rsimv _%I (_ _)%data_expr : assert.
 End sim_GS.
