theories/data_lang/semantics.v
@@ -1,0 +1,169 @@
+From simuliris Require Import
+  prelude.
+From simuliris.data_lang Require Export
+  syntax.
+From simuliris.data_lang Require Import
+  notations.
+
+Definition data_state := gmap loc data_val.
+
+#[global] Instance data_state_eq_dec :
+  EqDecision data_state.
+Proof.
+  solve_decision.
+Defined.
+#[global] Instance data_state_inhabited :
+  Inhabited data_state.
+Proof.
+  apply _.
+Qed.
+
+Implicit Types b : bool.
+Implicit Types l : loc.
+Implicit Types func : data_function.
+Implicit Types tag : data_tag.
+Implicit Types idx : data_index.
+Implicit Types v w : data_val.
+Implicit Types e : data_expr.
+Implicit Types prog : data_program.
+Implicit Types σ : data_state.
+
+Definition data_unop_eval op v :=
+  match op, v with
+  | DataOpNeg, DataBool b =>
+      Some (DataBool (negb b))
+  | DataOpUminus, DataInt n =>
+      Some (DataInt (- n))
+  | _, _ =>
+      None
+  end.
+#[global] Arguments data_unop_eval !_ !_ / : assert.
+
+Definition data_binop_eval_int op n1 n2 :=
+  match op with
+  | DataOpPlus =>
+      Some (DataInt (n1 + n2))
+  | DataOpMinus =>
+      Some (DataInt (n1 - n2))
+  | DataOpMult =>
+      Some (DataInt (n1 * n2))
+  | DataOpQuot =>
+      Some (DataInt (n1 `quot` n2))
+  | DataOpRem =>
+      Some (DataInt (n1 `rem` n2))
+  | DataOpLe =>
+      Some (DataBool (bool_decide (n1 ≤ n2)%Z))
+  | DataOpLt =>
+      Some (DataBool (bool_decide (n1 < n2)%Z))
+  | DataOpEq =>
+      Some (DataBool (bool_decide (n1 = n2)%Z))
+  end.
+#[global] Arguments data_binop_eval_int !_ _ _ / : assert.
+
+Definition data_binop_eval_bool op b1 b2 :=
+  match op with
+  | DataOpEq =>
+      Some (DataBool (bool_decide (b1 = b2)))
+  | _ =>
+      None
+  end.
+#[global] Arguments data_binop_eval_bool !_ _ _ / : assert.
+
+Definition data_binop_eval_function op func1 func2 :=
+  match op with
+  | DataOpEq =>
+      Some (DataBool (bool_decide (func1 = func2)))
+  | _ =>
+      None
+  end.
+#[global] Arguments data_binop_eval_function !_ _ _ / : assert.
+
+Definition data_binop_eval op v1 v2 :=
+  match v1, v2 with
+  | DataInt n1, DataInt n2 =>
+      data_binop_eval_int op n1 n2
+  | DataBool b1, DataBool b2 =>
+      data_binop_eval_bool op b1 b2
+  | DataFunc func1, DataFunc func2 =>
+      data_binop_eval_function op func1 func2
+  | _, _ =>
+      None
+  end.
+#[global] Arguments data_binop_eval !_ !_ !_ / : assert.
+
+Inductive data_head_step prog : data_expr → data_state → data_expr → data_state → Prop :=
+  | data_head_step_let v e e' σ :
+      e' = e.[#v/] →
+      data_head_step prog
+        (let: v in e) σ
+        e' σ
+  | data_head_step_call func v e e' σ :
+      prog !! func = Some e →
+      e' = e.[#v/] →
+      data_head_step prog
+        (func v) σ
+        e' σ
+  | data_head_step_unop op v v' σ :
+      data_unop_eval op v = Some v' →
+      data_head_step prog
+        (DataUnop op v) σ
+        v' σ
+  | data_head_step_binop_1 op e1 e2 e' σ :
+      e' = (let: e1 in let: e2.[ren (+1)] in DataBinopDet op $1 $0)%data_expr →
+      data_head_step prog
+        (DataBinop op e1 e2) σ
+        e' σ
+  | data_head_step_binop_2 op e1 e2 e' σ :
+      e' = (let: e2 in let: e1.[ren (+1)] in DataBinopDet op $0 $1)%data_expr →
+      data_head_step prog
+        (DataBinop op e1 e2) σ
+        e' σ
+  | data_head_step_binop_det op v1 v2 v' σ :
+      data_binop_eval op v1 v2 = Some v' →
+      data_head_step prog
+        (DataBinopDet op v1 v2) σ
+        v' σ
+  | data_head_step_if b e1 e2 σ :
+      data_head_step prog
+        (if: b then e1 else e2) σ
+        (if b then e1 else e2) σ
+  | data_head_step_constr_1 tag e1 e2 e' σ :
+      e' = (let: e1 in let: e2.[ren (+1)] in &&tag $1 $0)%data_expr →
+      data_head_step prog
+        (&tag e1 e2) σ
+        e' σ
+  | data_head_step_constr_2 tag e1 e2 e' σ :
+      e' = (let: e2 in let: e1.[ren (+1)] in &&tag $0 $1)%data_expr →
+      data_head_step prog
+        (&tag e1 e2) σ
+        e' σ
+  | data_head_step_constr_det tag v1 v2 σ l :
+      σ !! (l +ₗ 0) = None →
+      σ !! (l +ₗ 1) = None →
+      σ !! (l +ₗ 2) = None →
+      data_head_step prog
+        (&&tag v1 v2) σ
+        l (<[l +ₗ 2 := v2]> (<[l +ₗ 1 := v1]> (<[l +ₗ 0 := DataTag tag]> σ)))
+  | data_head_step_load l l' idx v σ :
+      σ !! (l +ₗ idx) = Some v →
+      data_head_step prog
+        (![idx] l) σ
+        v σ
+  | data_head_step_store l idx v w σ :
+      σ !! (l +ₗ idx) = Some v →
+      data_head_step prog
+        (l <-[idx]- w) σ
+        #() (<[l +ₗ idx := w]> σ).
+
+Lemma data_head_step_constr_det' prog tag v1 v2 σ σ' :
+  let l := loc_fresh (dom σ) in
+  σ' = <[l +ₗ 2 := v2]> (<[l +ₗ 1 := v1]> (<[l +ₗ 0 := DataTag tag]> σ)) →
+  data_head_step prog
+    (&&tag v1 v2) σ
+    l σ'.
+Proof.
+  intros l ->.
+  apply data_head_step_constr_det;
+    rewrite -not_elem_of_dom;
+    apply loc_fresh_fresh; lia.
+Qed.
