theories/data_lang/syntax.v
@@ -1,0 +1,236 @@
+From stdpp Require Export
+  strings
+  gmap.
+From stdpp Require Import
+  countable.
+
+From simuliris Require Import
+  prelude.
+From simuliris.common Require Export
+  autosubst
+  three
+  loc
+  typeclasses.
+
+Notation data_index := three (only parsing).
+
+Definition data_tag := nat.
+
+Notation data_function := string (only parsing).
+
+Inductive data_val :=
+  | DataUnit
+  | DataIndex (idx : data_index)
+  | DataTag (tag : data_tag)
+  | DataInt (n : Z)
+  | DataBool (b : bool)
+  | DataLoc (l : loc)
+  | DataFunc (func : data_function).
+
+#[global] Instance data_val_inhabited : Inhabited data_val :=
+  populate DataUnit.
+#[global] Instance data_val_eq_dec : EqDecision data_val :=
+  ltac:(solve_decision).
+#[global] Instance data_val_countable :
+  Countable data_val.
+Proof.
+  pose encode v :=
+    match v with
+    | DataUnit =>
+        inl ()
+    | DataIndex idx =>
+        inr $ inl idx
+    | DataTag tag =>
+        inr $ inr $ inl tag
+    | DataInt n =>
+        inr $ inr $ inr $ inl n
+    | DataBool b =>
+        inr $ inr $ inr $ inr $ inl b
+    | DataLoc l =>
+        inr $ inr $ inr $ inr $ inr $ inl l
+    | DataFunc func =>
+        inr $ inr $ inr $ inr $ inr $ inr func
+    end.
+  pose decode v :=
+    match v with
+    | inl () =>
+        DataUnit
+    | inr (inl idx) =>
+        DataIndex idx
+    | inr (inr (inl tag)) =>
+        DataTag tag
+    | inr (inr (inr (inl n))) =>
+        DataInt n
+    | inr (inr (inr (inr (inl b)))) =>
+        DataBool b
+    | inr (inr (inr (inr (inr (inl l))))) =>
+        DataLoc l
+    | inr (inr (inr (inr (inr (inr func))))) =>
+        DataFunc func
+    end.
+  apply (inj_countable' encode decode). intros []; done.
+Qed.
+
+#[global] Instance data_val_similar : Similar data_val data_val :=
+  Build_Similar $ λ v1 v2,
+    match v1, v2 with
+    | DataUnit, DataUnit =>
+        True
+    | DataIndex idx1, DataIndex idx2 =>
+        idx1 = idx2
+    | DataTag tag1, DataTag tag2 =>
+        tag1 = tag2
+    | DataInt i1, DataInt i2 =>
+        i1 = i2
+    | DataBool b1, DataBool b2 =>
+        b1 = b2
+    | DataLoc _, DataLoc _ =>
+        True
+    | DataFunc func1, DataFunc func2 =>
+        func1 = func2
+    | _, _ =>
+        False
+    end.
+
+Inductive data_unop :=
+  | DataOpNeg
+  | DataOpUminus.
+
+#[global] Instance data_unop_eq_dec : EqDecision data_unop :=
+  ltac:(solve_decision).
+#[global] Instance data_unop_countable :
+  Countable data_unop.
+Proof.
+  pose encode op :=
+    match op with
+    | DataOpNeg => 0
+    | DataOpUminus => 1
+    end.
+  pose decode op :=
+    match op with
+    | 0 => DataOpNeg
+    | _ => DataOpUminus
+    end.
+  apply (inj_countable' encode decode). intros []; done.
+Qed.
+
+Inductive data_binop :=
+  | DataOpPlus | DataOpMinus | DataOpMult | DataOpQuot | DataOpRem
+  | DataOpLe | DataOpLt | DataOpEq.
+
+#[global] Instance data_binop_eq_dec : EqDecision data_binop :=
+  ltac:(solve_decision).
+#[global] Instance data_binop_countable :
+  Countable data_binop.
+Proof.
+  pose encode op :=
+    match op with
+    | DataOpPlus => 0
+    | DataOpMinus => 1
+    | DataOpMult => 2
+    | DataOpQuot => 3
+    | DataOpRem => 4
+    | DataOpLe => 5
+    | DataOpLt => 6
+    | DataOpEq => 7
+    end.
+  pose decode op :=
+    match op with
+    | 0 => DataOpPlus
+    | 1 => DataOpMinus
+    | 2 => DataOpMult
+    | 3 => DataOpQuot
+    | 4 => DataOpRem
+    | 5 => DataOpLe
+    | 6 => DataOpLt
+    | _ => DataOpEq
+    end.
+  apply (inj_countable' encode decode). intros []; done.
+Qed.
+
+Inductive data_expr :=
+  | DataVal (v : data_val)
+  | DataVar (x : var)
+  | DataLet (e1 : data_expr) (e2 : {bind data_expr})
+  | DataCall (e1 e2 : data_expr)
+  | DataUnop (op : data_unop) (e : data_expr)
+  | DataBinop (op : data_binop) (e1 e2 : data_expr)
+  | DataBinopDet (op : data_binop) (e1 e2 : data_expr)
+  | DataIf (e0 e1 e2 : data_expr)
+  | DataConstr (tag : data_tag) (e1 e2 : data_expr)
+  | DataConstrDet (tag : data_tag) (e1 e2 : data_expr)
+  | DataLoad (e1 e2 : data_expr)
+  | DataStore (e1 e2 e3 : data_expr).
+
+#[global] Instance data_expr_inhabited : Inhabited data_expr :=
+  populate (DataVal inhabitant).
+#[global] Instance data_expr_eq_dec : EqDecision data_expr :=
+  ltac:(solve_decision).
+#[global] Instance data_expr_countable :
+  Countable data_expr.
+Proof.
+  pose fix encode e :=
+    match e with
+    | DataVal v =>
+        GenLeaf (inl v)
+    | DataVar x =>
+        GenLeaf (inr $ inl x)
+    | DataLet e1 e2 =>
+        GenNode 0 [encode e1; encode e2]
+    | DataCall e1 e2 =>
+        GenNode 1 [encode e1; encode e2]
+    | DataUnop op e =>
+        GenNode 2 [GenLeaf (inr $ inr $ inl op); encode e]
+    | DataBinop op e1 e2 =>
+        GenNode 3 [GenLeaf (inr $ inr $ inr $ inl op); encode e1; encode e2]
+    | DataBinopDet op e1 e2 =>
+        GenNode 4 [GenLeaf (inr $ inr $ inr $ inl op); encode e1; encode e2]
+    | DataIf e0 e1 e2 =>
+        GenNode 5 [encode e0; encode e1; encode e2]
+    | DataConstr tag e1 e2 =>
+        GenNode 6 [GenLeaf (inr $ inr $ inr $ inr tag); encode e1; encode e2]
+    | DataConstrDet tag e1 e2 =>
+        GenNode 7 [GenLeaf (inr $ inr $ inr $ inr tag); encode e1; encode e2]
+    | DataLoad e1 e2 =>
+        GenNode 8 [encode e1; encode e2]
+    | DataStore e1 e2 e3 =>
+        GenNode 9 [encode e1; encode e2; encode e3]
+    end.
+  pose fix decode e :=
+    match e with
+    | GenLeaf (inl v) =>
+        DataVal v
+    | GenLeaf (inr (inl x)) =>
+        DataVar x
+    | GenNode 0 [e1; e2] =>
+        DataLet (decode e1) (decode e2)
+    | GenNode 1 [e1; e2] =>
+        DataCall (decode e1) (decode e2)
+    | GenNode 2 [GenLeaf (inr (inr (inl op))); e] =>
+        DataUnop op (decode e)
+    | GenNode 3 [GenLeaf (inr (inr (inr (inl op)))); e1; e2] =>
+        DataBinop op (decode e1) (decode e2)
+    | GenNode 4 [GenLeaf (inr (inr (inr (inl op)))); e1; e2] =>
+        DataBinopDet op (decode e1) (decode e2)
+    | GenNode 5 [e0; e1; e2] =>
+        DataIf (decode e0) (decode e1) (decode e2)
+    | GenNode 6 [GenLeaf (inr (inr (inr (inr tag)))); e1; e2] =>
+        DataConstr tag (decode e1) (decode e2)
+    | GenNode 7 [GenLeaf (inr (inr (inr (inr tag)))); e1; e2] =>
+        DataConstrDet tag (decode e1) (decode e2)
+    | GenNode 8 [e1; e2] =>
+        DataLoad (decode e1) (decode e2)
+    | GenNode 9 [e1; e2; e3] =>
+        DataStore (decode e1) (decode e2) (decode e3)
+    | _ =>
+        @inhabitant _ data_expr_inhabited
+    end.
+  apply (inj_countable' encode decode). intros e. induction e; simpl; congruence.
+Qed.
+
+#[global] Instance data_expr_ids : Ids data_expr. derive. Defined.
+#[global] Instance data_expr_rename : Rename data_expr. derive. Defined.
+#[global] Instance data_expr_subst : Subst data_expr. derive. Defined.
+#[global] Instance data_expr_subst_lemmas : SubstLemmas data_expr. derive. Qed.
+
+Definition data_program := gmap data_function data_expr.
