theories/data_lang/tactics.v
@@ -1,0 +1,216 @@
+From simuliris Require Import
+  prelude.
+From simuliris.common Require Import
+  tactics.
+From simuliris.data_lang Require Export
+  language.
+From simuliris.data_lang Require Import
+  ectx_decompositions
+  metatheory.
+
+Create HintDb data_lang.
+
+#[global] Hint Extern 0 (
+  reducible _ _ _
+) => (
+  eapply head_reducible_reducible
+) : data_lang.
+#[global] Hint Extern 0 (
+  head_reducible _ _ _
+) => (
+  eexists _, _; simpl
+) : data_lang.
+#[global] Hint Extern 1 (
+  data_head_step _ _ _ _ _
+) => (
+  econstructor
+) : data_lang.
+#[global] Hint Extern 1 (
+  ectx_language.head_step _ _ _ _ _
+) => (
+  econstructor
+) : data_lang.
+#[global] Hint Extern 0 (
+  data_head_step _ (DataConstrDet _ _ _) _ _ _
+) => (
+  eapply data_head_step_constr_det'
+) : data_lang.
+#[global] Hint Extern 0 (
+  ectx_language.head_step _ (DataConstrDet _ _ _) _ _ _
+) => (
+  eapply data_head_step_constr_det'
+) : data_lang.
+#[global] Hint Extern 0 (
+  pure_step _ _ _
+) => (
+  eapply pure_exec_pure_step; [apply _ |]
+) : data_lang.
+#[global] Hint Extern 0 (
+  pure_head_step _ _ _
+) => (
+  eapply pure_head_exec_pure_head_step; [apply _ |]
+) : data_lang.
+#[global] Hint Extern 0 (
+  strongly_stuck _ _
+) => (
+  eapply @is_strongly_stuck; [apply _ |]
+) : data_lang.
+#[global] Hint Extern 0 (
+  strongly_head_stuck _ _
+) => (
+  eapply @is_strongly_head_stuck; [apply _ |]
+) : data_lang.
+
+#[global] Hint Extern 1 (
+  sub_redexes_are_values _
+) => (
+  let Hdecomps := fresh "Hdecomps" in
+  intros ?* Hdecomps%data_ectx_decompositions_spec;
+    invert Hdecomps; first done;
+    decompose_elem_of_list; simplify
+) : data_lang.
+
+Ltac data_expr_simplifier :=
+  repeat_on_hyps ltac:(fun H =>
+    match type of H with
+    | data_val_well_formed _ ?v =>
+        solve [by destruct v]
+    | data_expr_well_formed _ _ =>
+        simpl in H; destruct_and? H
+    | data_expr_scope _ _ =>
+        simpl in H; destruct_and? H
+    end
+  );
+  try done.
+#[global] Hint Extern 0 => (
+  solve [data_expr_simplifier]
+) : data_lang.
+#[global] Hint Extern 1 (
+  data_expr_well_formed _ _
+) => (
+  progress data_expr_simplifier
+) : data_lang.
+#[global] Hint Extern 1 (
+  data_expr_scope _ _
+) => (
+  progress data_expr_simplifier
+) : data_lang.
+
+Ltac invert_data_head_step :=
+  repeat_on_hyps ltac:(fun H =>
+    let ty := type of H in
+    let ty := eval simpl in ty in
+    match ty with data_head_step _ ?e _ _ _ =>
+      try (is_var e; fail 1);
+      invert H
+    end
+  ).
+
+#[local] Ltac solve_strongly_head_stuck :=
+  split;
+  [ intros ?** ?** ?; invert_data_head_step; done
+  | auto with data_lang
+  ].
+#[global] Instance strongly_head_stuck_data_var prog x :
+  IsStronglyHeadStuck prog
+    True
+    (DataVar x).
+Proof.
+  solve_strongly_head_stuck.
+Qed.
+#[global] Instance strongly_head_stuck_data_call prog v1 v2 :
+  IsStronglyHeadStuck prog
+    (if v1 is DataFunc _ then False else True)
+    (DataCall (DataVal v1) (DataVal v2)).
+Proof.
+  solve_strongly_head_stuck.
+Qed.
+#[global] Instance strongly_head_stuck_data_unop prog op v :
+  IsStronglyHeadStuck prog
+    (data_unop_eval op v = None)
+    (DataUnop op (DataVal v)).
+Proof.
+  solve_strongly_head_stuck.
+Qed.
+#[global] Instance strongly_head_stuck_data_binop_det prog op v1 v2 :
+  IsStronglyHeadStuck prog
+    (data_binop_eval op v1 v2 = None)
+    (DataBinopDet op (DataVal v1) (DataVal v2)).
+Proof.
+  solve_strongly_head_stuck.
+Qed.
+#[global] Instance strongly_head_stuck_data_if prog v0 e1 e2 :
+  IsStronglyHeadStuck prog
+    (if v0 is DataBool _ then False else True)
+    (DataIf (DataVal v0) e1 e2).
+Proof.
+  solve_strongly_head_stuck.
+Qed.
+#[global] Instance strongly_head_stuck_data_load_1 prog v1 v2 :
+  IsStronglyHeadStuck prog
+    (if (v1, v2) is (DataLoc _, DataIndex _) then False else True)
+    (DataLoad (DataVal v1) (DataVal v2)).
+Proof.
+  solve_strongly_head_stuck.
+Qed.
+#[global] Instance strongly_head_stuck_data_store_1 prog v1 v2 v3 :
+  IsStronglyHeadStuck prog
+    (if (v1, v2) is (DataLoc _, DataIndex _) then False else True)
+    (DataStore (DataVal v1) (DataVal v2) (DataVal v3)).
+Proof.
+  solve_strongly_head_stuck.
+Qed.
+
+#[local] Ltac solve_pure_head_exec :=
+  intros ?; apply nsteps_once; constructor;
+  [ auto with data_lang
+  | intros; invert_data_head_step; auto
+  ].
+#[global] Instance pure_exec_data_let prog v e :
+  PureHeadExec prog 1
+    True
+    (DataLet (DataVal v) e)
+    e.[DataVal v/].
+Proof.
+  solve_pure_head_exec.
+Qed.
+#[global] Instance pure_exec_data_call prog func v e :
+  PureHeadExec prog 1
+    (prog !! func = Some e)
+    (DataCall (DataVal (DataFunc func)) (DataVal v))
+    e.[DataVal v/].
+Proof.
+  solve_pure_head_exec.
+Qed.
+#[global] Instance pure_exec_data_unop prog op v w :
+  PureHeadExec prog 1
+    (data_unop_eval op v = Some w)
+    (DataUnop op (DataVal v))
+    (DataVal w).
+Proof.
+  solve_pure_head_exec.
+Qed.
+#[global] Instance pure_exec_data_binop_det prog op v1 v2 w :
+  PureHeadExec prog 1
+    (data_binop_eval op v1 v2 = Some w)
+    (DataBinopDet op (DataVal v1) (DataVal v2))
+    (DataVal w).
+Proof.
+  solve_pure_head_exec.
+Qed.
+#[global] Instance pure_exec_data_if_true prog e1 e2 :
+  PureHeadExec prog 1
+    True
+    (DataIf (DataVal (DataBool true)) e1 e2)
+    e1.
+Proof.
+  solve_pure_head_exec.
+Qed.
+#[global] Instance pure_exec_data_if_false prog e1 e2 :
+  PureHeadExec prog 1
+    True
+    (DataIf (DataVal (DataBool false)) e1 e2)
+    e2.
+Proof.
+  solve_pure_head_exec.
+Qed.
