theories/tmc/metatheory.v
@@ -2,15 +2,15 @@ From simuliris Require Import
   prelude.
 From simuliris.common Require Import
   tactics.
-From simuliris.lambda_lang Require Export
+From simuliris.data_lang Require Export
   metatheory.
-From simuliris.lambda_lang Require Import
+From simuliris.data_lang Require Import
   notations.
 From simuliris.tmc Require Export
   definition.
 
 Section tmc.
-  Context (ξ : gmap lambda_function lambda_function).
+  Context (ξ : gmap data_function data_function).
 
   Lemma tmc_dir_refl e :
     tmc_dir ξ e e.
@@ -61,85 +61,85 @@ Section tmc.
     eauto using (proj2 tmc_subst).
   Qed.
 
-  Lemma lambda_expr_scope_tmc :
+  Lemma data_expr_scope_tmc :
     ( ∀ eₛ eₜ,
       tmc_dir ξ eₛ eₜ →
       ∀ scope,
-      lambda_expr_scope scope eₛ →
-      lambda_expr_scope scope eₜ
+      data_expr_scope scope eₛ →
+      data_expr_scope scope eₜ
     ) ∧ (
       ∀ dst idx eₛ eₜ,
       tmc_dps ξ dst idx eₛ eₜ →
       ∀ scope,
-      lambda_expr_scope scope dst →
-      lambda_expr_scope scope idx →
-      lambda_expr_scope scope eₛ →
-      lambda_expr_scope scope eₜ
+      data_expr_scope scope dst →
+      data_expr_scope scope idx →
+      data_expr_scope scope eₛ →
+      data_expr_scope scope eₜ
     ).
   Proof.
     apply tmc_ind; try naive_solver.
     - intros * Hdir1 IH1 Hdps2 IH2 scope (Hscope1 & Hscope2).
       simpl. split_and!; try naive_solver lia.
       apply IH2; try naive_solver lia.
-      apply lambda_expr_scope_lift1. done.
+      apply data_expr_scope_lift1. done.
     - intros * Hdir2 IH2 Hdps1 IH1 scope (Hscope1 & Hscope2).
       simpl. split_and!; try naive_solver lia.
       apply IH1; try naive_solver lia.
-      apply lambda_expr_scope_lift1. done.
+      apply data_expr_scope_lift1. done.
     - intros * Hdir1 IH1 Hdps2 IH2 scope Hdst Hidx (Hscope1 & Hscope2).
       split; first auto.
-      apply IH2; try done; apply lambda_expr_scope_lift1; done.
+      apply IH2; try done; apply data_expr_scope_lift1; done.
     - intros * Hξ Hdir IH -> scope Hdst Hidx (_ & Hwf).
-      simpl. split_and!; [eauto using lambda_expr_scope_lift1.. | lia].
+      simpl. split_and!; [eauto using data_expr_scope_lift1.. | lia].
     - intros * Hdir1 IH1 Hdps2 IH2 -> scope Hdst Hidx (Hwf1 & Hwf2).
       simpl. split_and!; try naive_solver lia.
-      + apply lambda_expr_scope_lift1. done.
-      + apply lambda_expr_scope_lift1. done.
-      + apply (lambda_expr_scope_le (S (S scope))); first lia.
-        apply lambda_expr_scope_lift1, IH2; try naive_solver lia.
-        apply lambda_expr_scope_lift1. done.
+      + apply data_expr_scope_lift1. done.
+      + apply data_expr_scope_lift1. done.
+      + apply (data_expr_scope_le (S (S scope))); first lia.
+        apply data_expr_scope_lift1, IH2; try naive_solver lia.
+        apply data_expr_scope_lift1. done.
     - intros * Hdir2 IH2 Hdps1 IH1 -> scope Hdst Hidx (Hwf1 & Hwf2).
       simpl. split_and!; try naive_solver lia.
-      + apply lambda_expr_scope_lift1. done.
-      + apply lambda_expr_scope_lift1. done.
-      + apply (lambda_expr_scope_le (S (S scope))); first lia.
-        apply lambda_expr_scope_lift1, IH1; try naive_solver lia.
-        apply lambda_expr_scope_lift1. done.
+      + apply data_expr_scope_lift1. done.
+      + apply data_expr_scope_lift1. done.
+      + apply (data_expr_scope_le (S (S scope))); first lia.
+        apply data_expr_scope_lift1, IH1; try naive_solver lia.
+        apply data_expr_scope_lift1. done.
   Qed.
-  Lemma lambda_expr_scope_tmc_dir scope eₛ eₜ :
+  Lemma data_expr_scope_tmc_dir scope eₛ eₜ :
     tmc_dir ξ eₛ eₜ →
-    lambda_expr_scope scope eₛ →
-    lambda_expr_scope scope eₜ.
+    data_expr_scope scope eₛ →
+    data_expr_scope scope eₜ.
   Proof.
-    eauto using (proj1 lambda_expr_scope_tmc).
+    eauto using (proj1 data_expr_scope_tmc).
   Qed.
-  Lemma lambda_expr_scope_tmc_dps scope dst idx eₛ eₜ :
+  Lemma data_expr_scope_tmc_dps scope dst idx eₛ eₜ :
     tmc_dps ξ dst idx eₛ eₜ →
-    lambda_expr_scope scope dst →
-    lambda_expr_scope scope idx →
-    lambda_expr_scope scope eₛ →
-    lambda_expr_scope scope eₜ.
+    data_expr_scope scope dst →
+    data_expr_scope scope idx →
+    data_expr_scope scope eₛ →
+    data_expr_scope scope eₜ.
   Proof.
-    eauto using (proj2 lambda_expr_scope_tmc).
+    eauto using (proj2 data_expr_scope_tmc).
   Qed.
 End tmc.
 
 #[export] Hint Resolve tmc_dir_refl : tmc.
 
-Lemma lambda_program_scope_tmc progₛ progₜ :
+Lemma data_program_scope_tmc progₛ progₜ :
   tmc progₛ progₜ →
-  lambda_program_scope progₛ →
-  lambda_program_scope progₜ.
+  data_program_scope progₛ →
+  data_program_scope progₜ.
 Proof.
-  intros tmc. rewrite /lambda_program_scope !map_Forall_lookup => Hscope func eₜ Hfuncₜ.
+  intros tmc. rewrite /data_program_scope !map_Forall_lookup => Hscope func eₜ Hfuncₜ.
   apply elem_of_dom_2 in Hfuncₜ as Hfuncₜ'. rewrite tmc.(tmc_dom) elem_of_union in Hfuncₜ'.
   destruct Hfuncₜ' as [Hfuncₛ%lookup_lookup_total_dom | (func_dir & Hξ)%elem_of_map_img].
   - edestruct tmc.(tmc_dirs) as (_eₜ & Hdir & Heq); first done.
-    eapply lambda_expr_scope_tmc_dir; last naive_solver.
+    eapply data_expr_scope_tmc_dir; last naive_solver.
     rewrite Heq in Hfuncₜ. naive_solver.
   - pose proof Hξ as Hfunc_dirₛ%elem_of_dom_2%(tmc.(tmc_ξ_dom))%lookup_lookup_total_dom.
     edestruct tmc.(tmc_dpss) as (eₜ' & Hdps & Heq); [done.. |].
     rewrite Hfuncₜ in Heq. injection Heq as ->.
-    repeat constructor. eapply lambda_expr_scope_tmc_dps; [naive_solver.. |].
-    apply (lambda_expr_scope_le 1); naive_solver lia.
+    repeat constructor. eapply data_expr_scope_tmc_dps; [naive_solver.. |].
+    apply (data_expr_scope_le 1); naive_solver lia.
 Qed.
